examples/refinement/LowComp.fst
@@ -1,10 +1,5 @@
 module LowComp
 
-module B = LowStar.Buffer
-module ST = FStar.HyperStack.ST
-module HS = FStar.HyperStack
-module U32 = FStar.UInt32
-
 open HighComp
 open FStar.HyperStack
 open FStar.HyperStack.ST
@@ -13,29 +8,40 @@ open LowStar.BufferOps
 open LowStar.Modifies
 
 
+module H = FStar.Monotonic.Heap
+module B = LowStar.Buffer
+module ST = FStar.HyperStack.ST
+module HS = FStar.HyperStack
+module U32 = FStar.UInt32
+module Map = FStar.Map
+module M = LowStar.Modifies
+
 
 type lstate = pointer mint * pointer mint
 
 val well_formed : HS.mem -> lstate -> GTot Type0
 let well_formed h = fun (r1, r2) -> live h r1 /\ live h r2 /\ disjoint r1 r2
 
-// To and from high- and low-level state
+// To and from high- and low-level state coercions
+
 val lstate_as_state : HS.mem -> lstate -> GTot state
 let lstate_as_state h  = fun (b1, b2) -> (B.get h b1 0, B.get h b2 0)
 
 
-val g_upd_preserves_well_formed : #a:Type -> h:HS.mem -> b1:pointer a{live h b1} -> b2:pointer a{live h b2} -> v:a ->
+val g_upd_preserves_live : #a:Type -> h:HS.mem -> b1:pointer a{live h b1} -> b2:pointer a{live h b2} -> v:a ->
    Lemma (let h' = g_upd b1 0 v h in modifies (loc_buffer b1) h h' /\ live h b1 /\ live h' b2)
                                 
-let g_upd_preserves_well_formed #a h b1 b2 v = 
+let g_upd_preserves_live #a h b1 b2 v = 
   let p = g_upd_seq_as_seq b1 (Seq.upd (as_seq h b1) 0 v) h in ()
 
 val state_as_lstate : h:HS.mem -> ls:lstate{well_formed h ls} -> state -> GTot HS.mem 
 let state_as_lstate h =
   function (r1, r2) -> function (v1, v2) ->
     let h' = g_upd r1 0 v1 h in
-    let p = g_upd_preserves_well_formed h r1 r2 v1 in
+    let p = g_upd_preserves_live h r1 r2 v1 in
     g_upd r2 0 v2 h'
+
+// Low type variations
 
 type lcomp 'a (c : comp 'a) =
     (ls:lstate) ->
@@ -46,21 +52,38 @@ type lcomp 'a (c : comp 'a) =
                    //modifies (loc_union (loc_buffer (fst ls)) (loc_buffer (snd ls))) h h' /\
                    (let s0 = lstate_as_state h ls in
                     let (x, s1) = c s0 in
-                    h' == state_as_lstate h ls s1 /\ x == r )))
+                    Map.equal (get_hmap h') (get_hmap (state_as_lstate h ls s1)) /\ x == r )))
 
 
-let lcomp_wp (a:Type) (wp : state -> (a * state -> Type) -> Type) (c : comp_wp a wp) =
+
+// This type uses the coercion from high state to low state. Verification of DSL fails with a first try. 
+let lcomp_wp1 (a:Type) (wp : state -> (a * state -> Type) -> Type) (c : comp_wp a wp) =
      (ls:lstate) ->
      Stack a
        (requires (fun h -> well_formed h ls))
        (ensures  (fun h r h' ->
                     well_formed h' ls /\
                     (let s0 = lstate_as_state h ls in
-                     wp s0 (fun _ -> True) /\ 
+                     wp s0 (fun _ -> True) ==> 
                      (let tls = state_as_lstate h ls in // XXX fails otherwise
                       let (x, s1) = c s0 in 
                       h' == tls s1 /\ x == r ))))
-                    
+
+
+// This is the variation currenlty used
+let lcomp_wp (a:Type) (wp : state -> (a * state -> Type) -> Type) (c : comp_wp a wp) =
+     (ls:lstate) ->
+     Stack a
+       (requires (fun h -> well_formed h ls))
+       (ensures  (fun h r h' ->
+                    well_formed h' ls /\
+                    modifies (loc_union (loc_buffer (fst ls)) (loc_buffer (snd ls))) h h' /\
+                    (let s0 = lstate_as_state h ls in
+                     wp s0 (fun _ -> True) ==>
+                     (let res = c s0 in
+                      snd res == lstate_as_state h' ls /\ fst res == r))))
+
+
 let lcomp_wp' (a:Type) (wp : state -> (a * state -> Type) -> Type) (c : comp_wp a wp) =
     (ls:lstate) ->
     Stack a
@@ -116,17 +139,23 @@ let lwrite i v = fun (b1, b2) -> if i = 0 then b1.(0ul) <- v else b2.(0ul) <- v
 val lread : i:nat{ i < 2 } -> lcomp_wp mint (read_wp i) (hread' i)
 let lread i = fun (b1, b2) -> if i = 0 then b1.(0ul) else b2.(0ul)
 
-let monotonic (#a: Type) (wp: hwp a) = forall (s: state) p1 p2. (forall x. p1 x ==> p2 x) ==>
-  wp s p1 ==> wp s p2
+let monotonic (#a: Type) (wp: hwp a) = 
+    forall (s: state) p1 p2. (forall x. p1 x ==> p2 x) ==> wp s p1 ==> wp s p2
 
 let lbind (#a:Type) (#b:Type)
   (#wp1: state -> (a * state -> Type) -> Type)
   (#wp2: a -> state -> (b * state -> Type) -> Type)
   (#c1:comp_wp a wp1) (#c2:(x:a -> comp_wp b (wp2 x)))
   (m: lcomp_wp a wp1 c1) (f: (x:a) -> lcomp_wp b (wp2 x) (c2 x)):
-    lcomp_wp b (bind_wp wp1 wp2) (hbind' c1 c2) =
-      fun s ->
-        assume (monotonic wp1);
-        let a = m s in let r = f a s in r
+  lcomp_wp b (bind_wp wp1 wp2) (hbind' c1 c2) =
+  fun s ->
+    assume (monotonic wp1);
+    let a = m s in let r = f a s in r
 
 
+// Versions of [lread] and [lwrite] with reif in spec
+val lwrite' : i:nat{ i < 2 } -> v:mint -> lcomp_wp unit (write_wp i v) (reify (HIGH?.put i v))
+let lwrite' i v = fun (b1, b2) -> if i = 0 then b1.(0ul) <- v else b2.(0ul) <- v
+
+val lread' : i:nat{ i < 2 } -> lcomp_wp mint (read_wp i) (reify (HIGH?.get i))
+let lread' i = fun (b1, b2) -> if i = 0 then b1.(0ul) else b2.(0ul)
